add proofs in BBNot.v

src/BBNot.v
@@ -12,14 +12,14 @@ Import Prenex Implicits.
 
 (* ===== bit_blast_not ===== *)
 
-Definition bit_blast_not1 (g: generator) (a:literal) : generator * cnf * literal :=
+Definition bit_blast_not1 (g: generator) (l:literal) : generator * cnf * literal :=
   let (g', r):= gen g in
   let cs := [::
-        [:: r; a]; [:: neg_lit r; neg_lit a]
+        [:: r; l]; [:: neg_lit r; neg_lit l]
             ] in (g', cs , r).
 
-Fixpoint bit_blast_not g a : generator * cnf * word :=
-  match a with
+Fixpoint bit_blast_not g ls : generator * cnf * word :=
+  match ls with
   | [::] => (g, [::], [::])
   | hd :: tl =>
     let '(g_hd, cs_hd, lrs_hd) := bit_blast_not1 g hd in
@@ -27,14 +27,14 @@ Fixpoint bit_blast_not g a : generator * cnf * word :=
     (g_tl, catrev cs_hd cs_tl, lrs_hd :: lrs_tl)
   end.
 
-Definition mk_env_not1 E g a : env * generator * cnf * literal :=
+Definition mk_env_not1 E g l : env * generator * cnf * literal :=
   let (g', r) := gen g in
-  let E' := env_upd E (var_of_lit r) (~~ (interp_lit E a)) in
-  let cs := [:: [:: r; a]; [:: neg_lit r; neg_lit a]] in
+  let E' := env_upd E (var_of_lit r) (~~ (interp_lit E l)) in
+  let cs := [:: [:: r; l]; [:: neg_lit r; neg_lit l]] in
   (E', g', cs, r).
 
-Fixpoint mk_env_not E g a : env * generator * cnf * word :=
-  match a with
+Fixpoint mk_env_not E g ls : env * generator * cnf * word :=
+  match ls with
   | [::] => (E, g, [::], [::])
   | hd :: tl =>
     let '(E_hd, g_hd, cs_hd, lrs_hd) := mk_env_not1 E g hd in
@@ -42,111 +42,198 @@ Fixpoint mk_env_not E g a : env * generator * cnf * word :=
     (E_tl, g_tl, catrev cs_hd cs_tl, lrs_hd :: lrs_tl)
   end.
 
-Lemma bit_blast_not1_correct :
-  forall g b br E l g' cs lr,
+Lemma bit_blast_not1_correct g b br E l g' cs lr :
     bit_blast_not1 g l = (g', cs, lr) ->
     enc_bit E l b ->
     interp_cnf E (add_prelude cs) ->
     br = ~~ b ->
     enc_bit E lr br.
 Proof.
-Admitted.
+  rewrite /bit_blast_not1 /enc_bit. case=> _ <- <- /=.
+  rewrite add_prelude_expand /= interp_lit_neg_lit /=. move/eqP ->.
+  move/andP => [Htt Hcs] ->; t_clear.
+  move: Hcs. by case (E g); case b. 
+Qed.
 
-Lemma bit_blast_not_correct :
-  forall g bs E ls g' cs lrs,
+Lemma bit_blast_not_correct g bs E ls g' cs lrs:
     bit_blast_not g ls = (g', cs, lrs) ->
     enc_bits E ls bs ->
     interp_cnf E (add_prelude cs) ->
     enc_bits E lrs (invB bs).
 Proof.
-Admitted.
+  elim: ls g bs E g' cs lrs.
+  - move=> g bs E g' cs lr /=. case=> _ <- <- /=.
+    rewrite enc_bits_nil_l. move/eqP ->. done.
+  - move=> ls_hd ls_tl IH g bs E g' cs lrs.
+    rewrite /bit_blast_not -/bit_blast_not. 
+    case Hbb_hd : (bit_blast_not1 g ls_hd) => [[g_hd cs_hd] lrs_hd].
+    case Hbb_tl : (bit_blast_not g_hd ls_tl) => [[g_tl cs_tl] lrs_tl].
+    case=> _ <- <-. case: bs => [| bs_hd bs_tl] //=.
+    rewrite !enc_bits_cons add_prelude_catrev.
+    move => /andP [Henc_hd Henc_tl] /andP [Hi_hd Hi_tl].
+    rewrite (bit_blast_not1_correct Hbb_hd Henc_hd Hi_hd) /=; try done.
+    exact: (IH _ _ _ _ _ _ Hbb_tl Henc_tl Hi_tl).
+Qed.
 
-Lemma mk_env_not1_is_bit_blast_not1 :
-  forall E g l E' g' cs lr,
+Lemma mk_env_not1_is_bit_blast_not1 E g l E' g' cs lr:
     mk_env_not1 E g l = (E', g', cs, lr) ->
     bit_blast_not1 g l = (g', cs, lr).
 Proof.
-Admitted.
+  rewrite /mk_env_not1 /bit_blast_not1; intros;
+    dite_hyps; dcase_hyps; subst; reflexivity.
+Qed.
 
-Lemma mk_env_not_is_bit_blast_not :
-  forall E g ls E' g' cs lrs,
+Lemma mk_env_not_is_bit_blast_not E g ls E' g' cs lrs:
     mk_env_not E g ls = (E', g', cs, lrs) ->
     bit_blast_not g ls = (g', cs, lrs).
 Proof.
-Admitted.
+  elim: ls E g E' g' cs lrs => [| ls_hd ls_tl IH] E g E' g' cs lrs.
+  - by case=> _ <- <- <-.
+  - rewrite /bit_blast_not -/bit_blast_not /mk_env_not -/mk_env_not.
+    case Hmk_hd : (mk_env_not1 E g ls_hd) => [[[E_hd g_hd] cs_hd] lrs_hd].
+    case Hmk_tl : (mk_env_not E_hd g_hd ls_tl) => [[[E_tl g_tl] cs_tl] lrs_tl].
+    rewrite (mk_env_not1_is_bit_blast_not1 Hmk_hd).
+    rewrite (IH _ _ _ _ _ _ Hmk_tl).
+    by case=> _ <- <- <-.
+Qed.
 
-Lemma mk_env_not1_newer_gen :
-  forall E g l E' g' cs lr,
+Lemma mk_env_not1_newer_gen E g l E' g' cs lr:
     mk_env_not1 E g l = (E', g', cs, lr) ->
     (g <=? g')%positive.
 Proof.
-Admitted.
+  rewrite /mk_env_not1 /=. case=> _ <- _ _.
+  by t_auto_newer.
+Qed.
 
-Lemma mk_env_not_newer_gen :
-  forall E g ls E' g' cs lrs,
+Lemma mk_env_not_newer_gen E g ls E' g' cs lrs:
     mk_env_not E g ls = (E', g', cs, lrs) ->
     (g <=? g')%positive.
 Proof.
-Admitted.
+  elim: ls E g E' g' cs lrs => [| ls_hd ls_tl IH] E g E' g' cs lrs.
+  - case=> _ <- _ _; by t_auto_newer.
+  - rewrite /mk_env_not -/mk_env_not.
+    case Hmk_hd : (mk_env_not1 E g ls_hd) => [[[E_hd g_hd] cs_hd] lrs_hd].
+    case Hmk_tl : (mk_env_not E_hd g_hd ls_tl) => [[[E_tl g_tl] cs_tl] lrs_tl].
+    case=> _ <- _ _.
+    move: (mk_env_not1_newer_gen Hmk_hd) => Hggh. 
+    move: (IH _ _ _ _ _ _ Hmk_tl) => Hghgt.
+    by apply: (pos_leb_trans Hggh Hghgt).
+Qed.
 
-Lemma mk_env_not1_newer_res :
-  forall E g l E' g' cs lr,
+Lemma mk_env_not1_newer_res E g l E' g' cs lr:
     mk_env_not1 E g l = (E', g', cs, lr) ->
     newer_than_lit g l ->
     newer_than_lit g' lr.
 Proof.
-Admitted.
+  rewrite /mk_env_not1 /=. case=> _ <- _ <-.
+  by t_auto_newer.
+Qed.
 
-Lemma mk_env_not_newer_res :
-  forall E g ls E' g' cs lrs,
+Lemma mk_env_not_newer_res E g ls E' g' cs lrs:
     mk_env_not E g ls = (E', g', cs, lrs) ->
     newer_than_lits g ls ->
     newer_than_lits g' lrs.
 Proof.
-Admitted.
+  elim: ls E g E' g' cs lrs => [| ls_hd ls_tl IH] E g E' g' cs lrs.
+  - case=> _ <- _ <-; by t_auto_newer.
+  - rewrite /mk_env_not -/mk_env_not.
+    case Hmk_hd : (mk_env_not1 E g ls_hd) => [[[E_hd g_hd] cs_hd] lrs_hd].
+    case Hmk_tl : (mk_env_not E_hd g_hd ls_tl) => [[[E_tl g_tl] cs_tl] lrs_tl].
+    case=> _ <- _ <- /=.
+    move/andP => [Hglh Hglt].
+    move: (mk_env_not1_newer_gen Hmk_hd) => Hggh.
+    move: (mk_env_not_newer_gen Hmk_tl) => Hghgt.
+    move: (mk_env_not1_newer_res Hmk_hd Hglh) => Hghlrh.
+    apply/andP; split.
+    + by apply (newer_than_lit_le_newer Hghlrh).
+    + move: (newer_than_lits_le_newer Hglt Hggh) => Hghlt.
+      exact: (IH _ _ _ _ _ _ Hmk_tl Hghlt).
+Qed.
 
-Lemma mk_env_not1_newer_cnf :
-  forall E g l E' g' cs lr,
+Lemma mk_env_not1_newer_cnf E g l E' g' cs lr:
     mk_env_not1 E g l = (E', g', cs, lr) ->
     newer_than_lit g l ->
     newer_than_cnf g' cs.
 Proof.
-Admitted.
+  rewrite /mk_env_not1 /=. case=> _ <- <- _.
+  by t_auto_newer.
+Qed.
 
-Lemma mk_env_not_newer_cnf :
-  forall E g ls E' g' cs lrs,
+Lemma mk_env_not_newer_cnf E g ls E' g' cs lrs:
     mk_env_not E g ls = (E', g', cs, lrs) ->
     newer_than_lits g ls ->
     newer_than_cnf g' cs.
 Proof.
-Admitted.
+  elim: ls E g E' g' cs lrs => [| ls_hd ls_tl IH] E g E' g' cs lrs.
+  - case=> _ <- <- _; by t_auto_newer.
+  - rewrite /mk_env_not -/mk_env_not.
+    case Hmk_hd : (mk_env_not1 E g ls_hd) => [[[E_hd g_hd] cs_hd] lrs_hd].
+    case Hmk_tl : (mk_env_not E_hd g_hd ls_tl) => [[[E_tl g_tl] cs_tl] lrs_tl].
+    case=> _ <- <- _ /=. move/andP => [Hglh Hglt].
+    rewrite newer_than_cnf_catrev. 
+    move: (mk_env_not_newer_gen Hmk_tl) => Hghgt.
+    apply/andP; split.
+    + move: (mk_env_not1_newer_cnf Hmk_hd Hglh) => Hghch.
+      by apply (newer_than_cnf_le_newer Hghch).
+    + move: (mk_env_not1_newer_gen Hmk_hd) => Hggh.
+      move: (newer_than_lits_le_newer Hglt Hggh) => Hghlt.
+      exact: (IH _ _ _ _ _ _ Hmk_tl Hghlt).
+Qed.
 
-Lemma mk_env_not1_preserve :
-  forall E g l E' g' cs lr,
+Lemma mk_env_not1_preserve E g l E' g' cs lr:
     mk_env_not1 E g l = (E', g', cs, lr) ->
     env_preserve E E' g.
 Proof.
-Admitted.
+  rewrite /mk_env_not1 /=. case=> <- _ _ _.
+  by t_auto_preserve.
+Qed.
 
-Lemma mk_env_not_preserve :
-  forall E g ls E' g' cs lrs,
+Lemma mk_env_not_preserve E g ls E' g' cs lrs:
     mk_env_not E g ls = (E', g', cs, lrs) ->
     env_preserve E E' g.
 Proof.
-Admitted.
+  elim: ls E g E' g' cs lrs => [| ls_hd ls_tl IH] E g E' g' cs lrs.
+  - case=> <- _ _ _; by t_auto_preserve.
+  - rewrite /mk_env_not -/mk_env_not.
+    case Hmk_hd : (mk_env_not1 E g ls_hd) => [[[E_hd g_hd] cs_hd] lrs_hd].
+    case Hmk_tl : (mk_env_not E_hd g_hd ls_tl) => [[[E_tl g_tl] cs_tl] lrs_tl].
+    case=> <- _ _ _ /=. 
+    move: (mk_env_not1_preserve Hmk_hd) => HEEhg.
+    move: (IH _ _ _ _ _ _ Hmk_tl) => HEhEtgh.
+    move: (mk_env_not1_newer_gen Hmk_hd) => Hggh.
+    apply (env_preserve_trans HEEhg).
+    exact: (env_preserve_le HEhEtgh Hggh).
+Qed.
 
-Lemma mk_env_not1_sat :
-  forall E g l E' g' cs lr,
+Lemma mk_env_not1_sat E g l E' g' cs lr:
     mk_env_not1 E g l = (E', g', cs, lr) ->
     newer_than_lit g l ->
     interp_cnf E' cs.
 Proof.
-Admitted.
+  rewrite /mk_env_not1 /=. case=> <- _ <- _ Hgl.
+  move: (newer_than_lit_neq Hgl) => Hngl /=.
+  rewrite !env_upd_eq !interp_lit_neg_lit.
+  rewrite (interp_lit_env_upd_neq _ _ Hngl).
+  by case (interp_lit E l).
+Qed.
 
-Lemma mk_env_not_sat :
-  forall E g ls E' g' cs lrs,
+Lemma mk_env_not_sat E g ls E' g' cs lrs:
     mk_env_not E g ls = (E', g', cs, lrs) ->
     newer_than_lits g ls ->
     interp_cnf E' cs.
 Proof.
-Admitted.
+  elim: ls E g E' g' cs lrs => [| ls_hd ls_tl IH] E g E' g' cs lrs.
+  - by case=> <- _ <- _. 
+  - rewrite /mk_env_not -/mk_env_not.
+    case Hmk_hd : (mk_env_not1 E g ls_hd) => [[[E_hd g_hd] cs_hd] lrs_hd].
+    case Hmk_tl : (mk_env_not E_hd g_hd ls_tl) => [[[E_tl g_tl] cs_tl] lrs_tl].
+    case=> <- _ <- _ /=. move/andP => [Hglh Hglt].
+    rewrite interp_cnf_catrev; apply/andP; split.
+    + move: (mk_env_not_preserve Hmk_tl) => HpEhEtgh.
+      move: (mk_env_not1_newer_cnf Hmk_hd Hglh) => Hghch.
+      rewrite (env_preserve_cnf HpEhEtgh Hghch).
+      exact: (mk_env_not1_sat Hmk_hd Hglh).
+    + apply: (IH _ _ _ _ _ _ Hmk_tl). 
+      move: (mk_env_not1_newer_gen Hmk_hd). 
+      by apply: newer_than_lits_le_newer.
+Qed.
